\documentclass{article}
\usepackage{epsfig}
\pagestyle{empty}
\begin{document}
$A$
\pagebreak

$y = Ax$
\pagebreak

$y = M^{-1}x$
\pagebreak

$M$
\pagebreak

$M^{-1}$
\pagebreak

$Ax = b$
\pagebreak

$x = A^{-1}b$
\pagebreak

$A^{-1}$
\pagebreak

$x_{k+1} = Lx_k + b$
\pagebreak

$L$
\pagebreak

$b = L \cdot a$
\pagebreak

$x:=x+b$
\pagebreak

$x = M^{-1}b$
\pagebreak

$B = A^{T}$
\pagebreak

$B = A^{H}$
\pagebreak

$ u : [0, 1] \rightarrow R\\ u'' = f\\ u(0) = u0\\ u(1) = u1 $
\pagebreak

$ u(x + h) = u(x) - u'(x)h + 1/2 u''(x)h^2 + O(h^3)\\ u(x - h) = u(x) + u'(x)h + 1/2 u''(x)h^2 + O(h^3) / +\\ ---------------------- \\ -u(x - h) + 2u(x) + -u(x + h) = -f(x)h^2 + O(h^3) $
\pagebreak

$x1, ..., xk, $
\pagebreak

$ h = 1 / (K + 1)$
\pagebreak

$ 2u_1 - u_2 = -f_1 h^2 + u0\\ -u_(k-1) + 2u_k - u_(k+1) = -f_k h^2, k = 2, ..., K - 1\\ -u_(K-1) + 2u_K = -f_K h^2 + u1\\ $
\pagebreak

$`f` $
\pagebreak

$`f(x) = 6x`$
\pagebreak

$`u(x) = x^3`$
\pagebreak

\end{document}
